assign 13

assignments/13/P05.v
@@ -13,30 +13,51 @@ Require Export P04.
 *)
 
 Definition halve : tm :=
-  GIVEUP.
+  tfix
+  (tabs K (TArrow TNat TNat) 
+    (tabs N TNat (tif0 (tvar N) (tnat 0)
+                   (tif0 (tpred (tvar N)) (tnat 0)
+                     (tsucc (tapp (tvar K) (tpred (tpred (tvar N))))))))).
+
 
 Example halve_type: empty |- halve \in TArrow TNat TNat.
 Proof.
-  (* unfold halve; eauto 10. *)
-  exact GIVEUP.
+   unfold halve; eauto 10. 
 Qed.
 
 Example halve_10: tapp halve (tnat 10) ==>* tnat 5.
 Proof.
-  (* unfold halve; normalize. *)
-  exact GIVEUP.
+   unfold halve; normalize. 
 Qed.
 
 Example halve_11: tapp halve (tnat 11) ==>* tnat 5.
 Proof.
-  (* unfold halve; normalize. *)
-  exact GIVEUP.
+   unfold halve; normalize. 
 Qed.
 
 
 Theorem halve_correct: forall n,
    tapp halve (tnat (n+n)) ==>* tnat n.
 Proof.
-  exact GIVEUP.
+ induction n.
+- unfold halve. normalize.
+- unfold halve in *. simpl. rewrite plus_comm. simpl.
+    eapply multi_step. apply ST_AppFix. auto. auto. 
+eapply multi_step. apply ST_App1. auto. simpl.
+eapply multi_step. apply ST_AppAbs. auto. simpl. 
+eapply multi_step. apply ST_If0Nonzero. 
+eapply multi_step. apply ST_If01. apply ST_PredNat. simpl. 
+eapply multi_step. apply ST_If0Nonzero. 
+eapply multi_step. apply ST_Succ1. apply ST_App2. auto. apply ST_Pred. apply ST_PredNat. simpl.
+    eapply multi_step. apply ST_Succ1. apply ST_App2. auto. apply ST_PredNat. simpl.
+
+
+ assert ( K: forall t t', t ==>* t' -> tsucc t ==>* tsucc t').
+    intros. induction H. constructor. 
+eapply multi_step. apply ST_Succ1. apply H. 
+assumption.     
+
+ eapply multi_trans. apply K. 
+apply IHn. eapply multi_step. apply ST_SuccNat. constructor.
 Qed.
 
