assignments/13/P01.v
@@ -8,6 +8,17 @@ Require Export D.
           empty |- \x:S. x x : T).
 *)
 
+Lemma K:
+  forall T1 T2, ~ T1 = TArrow T1 T2.
+Proof.
+  unfold not.
+  intros. generalize dependent T2. 
+  induction T1; intros; 
+  inversion H.
+  apply IHT1_1 in H1. assumption. 
+Qed.
+
+
 Example typing_nonexample_3 :
   ~ (exists S, exists T,
         empty |- 
@@ -15,6 +26,22 @@ Example typing_nonexample_3 :
              (tapp (tvar X) (tvar X))) \in
           T).
 Proof.
-  exact GIVEUP.
+  intros Hc.
+  destruct Hc.
+  destruct H. 
+ 
+  inversion H; subst. clear H.
+  inversion H5; subst. clear H5.
+  inversion H2; subst. clear H2. 
+  inversion H4; subst. clear H4.
+  
+  rewrite extend_eq in H1.
+  rewrite extend_eq in H2. rewrite H1 in H2. 
+  inversion H2. 
+   symmetry in H0. 
+  apply K in H0. 
+  assumption.
+
+
 Qed.
 
