assignments/13/P02.v
@@ -7,6 +7,12 @@ Corollary typable_empty__closed : forall t T,
     empty |- t \in T  ->
     closed t.
 Proof.
-  exact GIVEUP.
+ intros.
+  unfold closed.
+  unfold not. 
+  intros. 
+  apply free_in_context with (T := T) (Gamma :=\empty) in H0.  inversion H0.  inversion H1. apply H.  
+
+
 Qed.
 
