assignments/13/P03.v
@@ -12,6 +12,27 @@ Lemma type_is_unique: forall t G T T'
     (TYPED': G |- t \in T'),
   T = T'.
 Proof.
-  exact GIVEUP.
+ intros.
+ generalize dependent T'.
+ induction TYPED; intros;
+ inversion TYPED'; subst; auto. 
+ rewrite H in H2. inversion H2. 
+ auto. 
+ apply IHTYPED in H4. rewrite H4. auto. 
+ apply IHTYPED1 in H2. inversion H2; subst. auto.
+ apply IHTYPED1 in H2. apply IHTYPED2 in H4.
+ rewrite H2. rewrite H4. auto. 
+ apply IHTYPED in H1. inversion H1; subst. auto.   
+    apply IHTYPED in H1. inversion H1; subst.
+    auto.
+    apply IHTYPED1 in H4. subst. apply IHTYPED2 in H5. auto. 
+    apply IHTYPED in H3. rewrite H3. auto.
+    apply IHTYPED in H3. rewrite H3. auto.
+    apply IHTYPED1 in H6. inversion H6; subst.
+    apply IHTYPED2 in H7. auto.
+    apply IHTYPED in H1. inversion H1;subst.
+    auto. 
+
+
 Qed.
 
