assignments/13/P04.v
@@ -7,6 +7,20 @@ Corollary soundness : forall t t' T,
   t ==>* t' ->
   ~(stuck t').
 Proof.
-  exact GIVEUP.
+ unfold not, stuck. unfold not.
+ intros.
+    destruct H1. 
+    unfold normal_form in H1.
+    unfold not in H1. 
+    induction H0.
+    apply progress in H.
+    inversion H. apply H2 in H0. auto.
+    apply H1 in H0. auto. 
+    eapply preservation in H. 
+    apply IHmulti in H. auto. 
+    apply H1. apply H2. apply H0.   
+
+
+
 Qed.
 
